SeparationLogic/examples/Applications_human/alpha_equiv/thm_apply_proof_auto.v
@@ -196,21 +196,15 @@ Proof. Admitted.
 Lemma proof_of_thm_apply_partial_solve_wit_5 : thm_apply_partial_solve_wit_5.
 Proof. Admitted. 
 
-Lemma proof_of_thm_apply_partial_solve_wit_6_pure : thm_apply_partial_solve_wit_6_pure.
-Proof. Admitted. 
-
 Lemma proof_of_thm_apply_partial_solve_wit_6 : thm_apply_partial_solve_wit_6.
 Proof. Admitted. 
 
 Lemma proof_of_thm_apply_partial_solve_wit_7 : thm_apply_partial_solve_wit_7.
 Proof. Admitted. 
 
+Lemma proof_of_thm_apply_partial_solve_wit_8_pure : thm_apply_partial_solve_wit_8_pure.
+Proof. Admitted. 
+
 Lemma proof_of_thm_apply_partial_solve_wit_8 : thm_apply_partial_solve_wit_8.
-Proof. Admitted. 
-
-Lemma proof_of_thm_apply_partial_solve_wit_9_pure : thm_apply_partial_solve_wit_9_pure.
-Proof. Admitted. 
-
-Lemma proof_of_thm_apply_partial_solve_wit_9 : thm_apply_partial_solve_wit_9.
 Proof. Admitted. 
 
